pulse/ulib/experimental/Steel.PCM.HigherReference.fsti
@@ -25,6 +25,17 @@ val ref (a:Type u#1) : Type u#0
 
 val pts_to (#a:Type u#1) (r:ref a) (p:perm) (v:erased a) : slprop u#1
 
+val pts_to_ref_injective
+      (#a: Type u#1)
+      (r: ref a)
+      (p0 p1:perm)
+      (v0 v1: erased a)
+      (m:mem)
+    : Lemma
+      (requires
+        interp (pts_to r p0 v0 `star` pts_to r p1 v1) m)
+      (ensures v0 == v1)
+
 val alloc (#a:Type) (x:a)
   : SteelT (ref a) emp (fun r -> pts_to r full_perm x)
 
